theories/Trace.v
@@ -2,13 +2,17 @@ From MetaCoq.Utils Require Import MCUtils bytestring.
 From MetaCoq.Guarded Require Import Except util.
 Require Import List.
 
+Require Import BinNat.
+
+
 (** Trace Monad built on top of the exception monad for easier debugging. *)
 (** Provides means to limit the number of binds until timeout and to add trace information *)
 (** Sadly not very usable in practice due to slow Coq reduction. *)
 
-Definition TIMEOUT_TIME := 182.
-Definition TIMEOUT := true.
+Definition TIMEOUT_TIME := 3000%N.
+Definition TIMEOUT := false.
 Definition TRACE := true.
+
 Notation "'fast_if' c 'then' u 'else' v" :=
   (ltac:(let x := eval cbv in c in
          match x with
@@ -19,14 +23,14 @@ Notation "'fast_if' c 'then' u 'else' v" :=
 
 (* Check (fast_if true then 1 else 0). *)
 Section trace.
-  Context (max_steps : nat).
+  Context (max_steps : N).
   Context {Y : Type}.
   Context (timeout : Y).
 
   Definition trace_info := string.
   Open Scope type_scope.
   Definition TraceM A :=  bool (* timeout *)
-                        * nat (* number of steps on the clock *)
+                        * N (* number of steps on the clock *)
                         * list trace_info (* trace *)
                         * excOn Y A.
   
@@ -34,7 +38,7 @@ Section trace.
   (* max steps handling is not totally accurate as we cannot pass the current number of steps into the function in bind, but anyways *)
   Instance trace_monad : Monad TraceM :=
     {|
-      ret := fun T t => (false, 0, [], ret t);
+      ret := fun T t => (false, 0%N, [], ret t);
       bind := fun T U (x : TraceM T) (f : T -> TraceM U) => 
         match x with
         | (b, s, t, e) =>
@@ -50,33 +54,46 @@ Section trace.
                 end
             | inr err => (false, s, t, inr err)
             end *)
-            let res := match e with
-              | inl e =>
-                  match f e return TraceM U with
-                  | (b', s', t', e') =>
-                      let s'' := (fast_if TIMEOUT then 1 + s' + s else 0) in
-                      let t'' := (fast_if TRACE then t' ++ t else @nil trace_info) in
-                      let terminate := andb TIMEOUT $ orb b (Nat.leb max_steps s'') in
-                      (terminate, s'', t'', e')
-                  end
-              | inr err => (false, s, t, inr err)
-              end
-            in fast_if TIMEOUT then (if b then (b, s, t, raise timeout) else res) else res
-        end
+            fast_if TIMEOUT then
+              if b then (b, s, t, raise timeout) else 
+                match e with
+                | inl e =>
+                    match f e return TraceM U with
+                    | (b', s', t', e') =>
+                        let s'' := (fast_if TIMEOUT then 1 + s' + s else 0)%N in
+                        let t'' := (fast_if TRACE then t' ++ t else @nil trace_info) in
+                        let terminate := andb TIMEOUT $ orb b (N.leb max_steps s'') in
+                        (terminate, s'', t'', e')
+                    end
+                | inr err => (false, s, t, inr err)
+                end
+            else
+                match e with
+                | inl e =>
+                    match f e return TraceM U with
+                    | (b', s', t', e') =>
+                        let s'' := (fast_if TIMEOUT then 1 + s' + s else 0)%N in
+                        let t'' := (fast_if TRACE then t' ++ t else @nil trace_info) in
+                        let terminate := andb TIMEOUT $ orb b (N.leb max_steps s'') in
+                        (terminate, s'', t'', e')
+                    end
+                | inr err => (false, s, t, inr err)
+                end
+      end
     |}.
 
   (* emit a trace element *)
   Definition trace (i : trace_info) : TraceM unit :=
-    (false, 0, fast_if TRACE then [i] else @nil trace_info, ret tt).
+    (false, 0, fast_if TRACE then [i] else @nil trace_info, ret tt)%N.
   Definition step : TraceM unit :=
-    (false, fast_if TIMEOUT then 1 else 0, [], ret tt).
+    (false, fast_if TIMEOUT then 1 else 0, [], ret tt)%N.
 
 
   (** Lifting of the primitive operations on the except monad *)
   Notation "'trc' A" := (@TraceM A) (at level 100).
 
-  Definition raise {X} (y : Y) : trc X := (false, 0, [], Except.raise y).
-  Definition except {X} (y: Y) (a : option X) : trc X := (false, 0, [], Except.except y a).
+  Definition raise {X} (y : Y) : trc X := (false, 0, [], Except.raise y)%N.
+  Definition except {X} (y: Y) (a : option X) : trc X := (false, 0, [], Except.except y a)%N.
 
   Class TrcUnwrap (Xl : Type -> Type) := trc_unwrap X : Xl (trc X) -> trc (Xl X).
   Arguments trc_unwrap {_ _ _}.
@@ -91,8 +108,8 @@ Section trace.
     end.
   Instance list_trc_unwrap: TrcUnwrap list := @list_unwrap.
 
-  Definition lift_exc {X} (a : excOn Y X) : trc X := (false, 0, [], a).
-  Definition add_trace {Z} (steps : nat) trace (a : trc Z) :=
+  Definition lift_exc {X} (a : excOn Y X) : trc X := (false, 0, [], a)%N.
+  Definition add_trace {Z} (steps : N) trace (a : trc Z) :=
     match a with
     | (b', steps', trace', z) =>
         (* if (andb TIMEOUT b') then (b', steps', trace', z) else
@@ -101,12 +118,12 @@ Section trace.
         let terminate := andb TIMEOUT $ orb b' (Nat.leb max_steps s) in
         (terminate, s, t, z) *)
         let res := 
-          let s := fast_if TIMEOUT then 1 + steps' + steps else 0 in
+          let s := (fast_if TIMEOUT then 1 + steps' + steps else 0) in
           let t := fast_if TRACE then trace' ++ trace else @nil trace_info in
-          let terminate := andb TIMEOUT $ orb b' (Nat.leb max_steps s) in
+          let terminate := andb TIMEOUT $ orb b' (N.leb max_steps s) in
           (terminate, s, t, z)
         in fast_if TIMEOUT then (if b' then (b', steps', trace', z) else res) else res
-    end.
+    end%N.
 
   Definition assert (b : bool) (err : Y) : trc unit :=
     lift_exc (Except.assert b err).
@@ -146,34 +163,34 @@ Section trace.
     Defined.
 
 End trace.
-Check (catchMap : nat -> forall Y : Type, Y -> forall X Z : Type, TraceM X -> (Y -> TraceM Z) -> (X -> TraceM Z) -> TraceM Z).
+Check (catchMap : N -> forall Y : Type, Y -> forall X Z : Type, TraceM X -> (Y -> TraceM Z) -> (X -> TraceM Z) -> TraceM Z).
 
 Arguments trc_unwrap {_ _ _ _}.
 
-Module example.
-  Inductive err :=
-  | TimeoutErr
-  | OtherErr (s : string).
+(* Module example. *)
+(*   Inductive err := *)
+(*   | TimeoutErr *)
+(*   | OtherErr (s : string). *)
 
-  Definition max_steps := 2.
-  Definition catchE := @catchE max_steps.
-  Arguments catchE {_ _}.
+(*   Definition max_steps := 2%N. *)
+(*   Definition catchE := @catchE max_steps. *)
+(*   Arguments catchE {_ _}. *)
 
-  (* Instance: Monad (@TraceM err) := @trace_monad max_steps err. *)
-  Instance: Monad (@TraceM err).
-  Proof.
-    apply trace_monad.
-    all: (apply max_steps || apply TimeoutErr).
-  Defined.
+(*   (* Instance: Monad (@TraceM err) := @trace_monad max_steps err. *) *)
+(*   Instance: Monad (@TraceM err). *)
+(*   Proof. *)
+(*     apply trace_monad. *)
+(*     all: (apply max_steps || apply TimeoutErr). *)
+(*   Defined. *)
 
-  Notation "'trc' A" := (@TraceM err A) (at level 100).
+(*   Notation "'trc' A" := (@TraceM err A) (at level 100). *)
 
-  Open Scope string_scope.
-  Definition test : trc unit :=
-    trace "test"%bs;;
-    raise $ OtherErr "s"%bs.
+(*   Open Scope string_scope. *)
+(*   Definition test : trc unit := *)
+(*     trace "test"%bs;; *)
+(*     raise $ OtherErr "s"%bs. *)
 
-  Definition test' : trc unit :=
-    catchE test (fun _ => step;; raise $ OtherErr "sss"%bs).
-  (*Eval cbn in test'.*)
-End example.
+(*   Definition test' : trc unit := *)
+(*     catchE test (fun _ => step;; raise $ OtherErr "sss"%bs). *)
+(*   (*Eval cbn in test'.*) *)
+(* End example. *)
